examples/miniML/hol2miniml/other-examples/example_parser_genScript.sml
@@ -14,59 +14,6 @@ val EqualityType_CHAR = prove(
   ``EqualityType CHAR``,
   EVAL_TAC THEN SRW_TAC [] [] THEN EVAL_TAC) |> store_eq_thm;
 
-
-(* register ptree -- begin *)
-
-val _ = register_type ``:'a list``
-
-(*
-
-val list_CONG = store_thm("list_CONG",
-  ``!l1 l2 P P'.
-      (l1 = l2) /\ (!x. MEM x l2 ==> (P x = P' x)) ==>
-      (list P l1 = list P' l2)``,
-  Induct THEN Cases_on `l2` THEN SIMP_TAC (srw_ss()) [FUN_EQ_THM]
-  THEN ONCE_REWRITE_TAC [fetch "-" "list_def"]
-  THEN SIMP_TAC std_ss [] THEN METIS_TAC []);
-
-*)
-
-(* val _ = register_type ``:ptree`` *)
-
-val ty = ``:ptree``
-
-val _ = delete_const "ptree" handle _ => ()
-
-val tm =
-  ``(ptree (Leaf x1_1) v ⇔
-   ∃v1_1. (v = Conv "Leaf" [v1_1]) ∧ list CHAR x1_1 v1_1) ∧
-  (ptree (Node x2_1 x2_2) v ⇔
-   ∃v2_1 v2_2.
-     (v = Conv "Node" [v2_1; v2_2]) ∧ list CHAR x2_1 v2_1 ∧
-     list (\x v. if MEM x x2_2 then ptree x v else ARB) x2_2 v2_2)``
-
-val inv_def = tDefine "ptree_def" [ANTIQUOTE tm]
- (WF_REL_TAC `measure (ptree_size o FST)`
-  THEN STRIP_TAC THEN Induct
-  THEN EVAL_TAC THEN SIMP_TAC std_ss []
-  THEN REPEAT STRIP_TAC THEN RES_TAC
-  THEN FULL_SIMP_TAC std_ss [] THEN DECIDE_TAC)
-
-val list_SIMP = prove(
-  ``!xs b. list (\x v. if b x \/ MEM x xs then p x v else q) xs = list p xs``,
-  Induct
-  THEN FULL_SIMP_TAC std_ss [FUN_EQ_THM,fetch "-" "list_def",MEM,DISJ_ASSOC])
-  |> Q.SPECL [`xs`,`\x.F`] |> SIMP_RULE std_ss [];
-
-val inv_def = inv_def |> SIMP_RULE std_ss [list_SIMP]
-                      |> CONV_RULE (DEPTH_CONV ETA_CONV)
-
-val _ = set_inv_def (ty,inv_def)
-
-val _ = register_type ``:ptree``
-
-(* register ptree -- end *)
-
 val res = translate listTheory.HD;
 val res = translate listTheory.TL;
 val res = translate listTheory.LENGTH;
